Utilisation d'un intermédiaire xfunction contenant le revmap

backend/Duplicate.v
@@ -1,48 +1,68 @@
 (** RTL node duplication using external oracle. Used to form superblock
   structures *)
 
-Require Import AST RTL Maps.
+Require Import AST RTL Maps Globalenvs.
 Require Import Coqlib Errors.
 
 Local Open Scope error_monad_scope.
 
 (** External oracle returning the new RTL code (entry point unchanged),
     along with the new entrypoint, and a mapping of new nodes to old nodes *)
-Axiom duplicate_aux: RTL.function -> RTL.code * node * (PTree.t nat).
+Axiom duplicate_aux: function -> code * node * (PTree.t node).
 
 Extract Constant duplicate_aux => "Duplicateaux.duplicate_aux".
+
+Record xfunction : Type := 
+ { fn_RTL: function;
+   fn_revmap: PTree.t node;
+ }.
+
+Definition xfundef := AST.fundef xfunction.
+Definition xprogram := AST.program xfundef unit.
+Definition xgenv := Genv.t xfundef unit.
+
+Definition fundef_RTL (fu: xfundef) : fundef := 
+  match fu with
+  | Internal f => Internal (fn_RTL f)
+  | External ef => External ef
+  end.
 
 (** * Verification of node duplications *)
 
 (** Verifies that the mapping [mp] is giving correct information *)
-Definition verify_mapping (f: function) (tc: code) (tentry: node) (mp: PTree.t nat) : res unit := OK tt. (* TODO *)
+Definition verify_mapping (xf: xfunction) (tc: code) (tentry: node) : res unit := OK tt. (* TODO *)
 
 (** * Entry points *)
 
-Definition transf_function (f: function) : res function :=
+Definition transf_function (f: function) : res xfunction :=
   let (tcte, mp) := duplicate_aux f in
   let (tc, te) := tcte in
-  do u <- verify_mapping f tc te mp;
-  OK (mkfunction (fn_sig f) (fn_params f) (fn_stacksize f) tc te).
+  let xf := {| fn_RTL := (mkfunction (fn_sig f) (fn_params f) (fn_stacksize f) tc te); fn_revmap := mp |} in
+  do u <- verify_mapping xf tc te;
+  OK xf.
 
 Theorem transf_function_preserves:
-  forall f tf,
-  transf_function f = OK tf ->
-     fn_sig f = fn_sig tf /\ fn_params f = fn_params tf /\ fn_stacksize f = fn_stacksize tf.
+  forall f xf,
+  transf_function f = OK xf ->
+     fn_sig f = fn_sig (fn_RTL xf) /\ fn_params f = fn_params (fn_RTL xf) /\ fn_stacksize f = fn_stacksize (fn_RTL xf).
 Proof.
   intros. unfold transf_function in H. destruct (duplicate_aux _) as (tcte & mp). destruct tcte as (tc & te). monadInv H.
   repeat (split; try reflexivity).
 Qed.
 
-Remark transf_function_fnsig: forall f tf, transf_function f = OK tf -> fn_sig f = fn_sig tf.
+Remark transf_function_fnsig: forall f xf, transf_function f = OK xf -> fn_sig f = fn_sig (fn_RTL xf).
   Proof. apply transf_function_preserves. Qed.
-Remark transf_function_fnparams: forall f tf, transf_function f = OK tf -> fn_params f = fn_params tf.
+Remark transf_function_fnparams: forall f xf, transf_function f = OK xf -> fn_params f = fn_params (fn_RTL xf).
   Proof. apply transf_function_preserves. Qed.
-Remark transf_function_fnstacksize: forall f tf, transf_function f = OK tf -> fn_stacksize f = fn_stacksize tf.
+Remark transf_function_fnstacksize: forall f xf, transf_function f = OK xf -> fn_stacksize f = fn_stacksize (fn_RTL xf).
   Proof. apply transf_function_preserves. Qed.
 
-Definition transf_fundef (f: fundef) : res fundef :=
+Definition transf_fundef_aux (f: fundef) : res xfundef :=
   transf_partial_fundef transf_function f.
+
+Definition transf_fundef (f: fundef): res fundef :=
+  do xf <- transf_fundef_aux f;
+  OK (fundef_RTL xf).
 
 Definition transf_program (p: program) : res program :=
   transform_partial_program transf_fundef p.
